ps2.

pset01_ProgramAnalysis/Pset1Implementation.v
@@ -19,8 +19,11 @@ Module Impl.
   (* Define [Neg] so that it implements Boolean negation, which flips
    * the truth value of a Boolean value.
    *)
-  Definition Neg (b : bool) : bool.
-  Admitted.
+  Definition Neg (b : bool) : bool :=
+    match b with
+    | true => false
+    | false => true
+    end.
 
   (* For instance, the negation of [true] should be [false].
    * This proof should follow from reducing both sides of the equation
@@ -28,7 +31,8 @@ Module Impl.
    *)
   Theorem Neg_true : Neg true = false.
   Proof.
-  Admitted.
+    simplify; equality.
+  Qed.
 
   (* Negation should be involutive, meaning that if we negate
    * any Boolean value twice, we should get the original value back.
@@ -39,39 +43,54 @@ Module Impl.
    *)
   Theorem Neg_involutive : forall b : bool, Neg (Neg b) = b.
   Proof.
-  Admitted.
+    simplify.
+    cases b.
+    simplify; equality.
+    simplify; equality.
+  Qed.
 
   (* Define [And] so that it implements Boolean conjunction. That is,
    * the result value should be [true] exactly when both inputs
    * are [true].
    *)
-  Definition And (x y : bool) : bool.
-  Admitted.
+  Definition And (x y : bool) : bool :=
+    match (x, y) with
+    | (true, true) => true
+    | (_, _) => false
+    end.
 
   (* Here are a couple of examples of how [And] should act on
    * concrete inputs.
    *)
   Theorem And_true_true : And true true = true.
   Proof.
-  Admitted.
+    simplify. equality.
+  Qed.
 
   Theorem And_false_true : And false true = false.
   Proof.
-  Admitted.
+    simplify. equality.
+  Qed.
 
   (* Prove that [And] is commutative, meaning that switching the order
    * of its arguments doesn't affect the result.
    *)
   Theorem And_comm : forall x y : bool, And x y = And y x.
   Proof.
-  Admitted.
+    induct x.
+    simplify. equality.
+    simplify. induct y. simplify. equality. equality.
+  Qed.
 
   (* Prove that the conjunction of a Boolean value with [true]
    * doesn't change that value.
    *)
   Theorem And_true_r : forall x : bool, And x true = x.
   Proof.
-  Admitted.
+    induct x.
+    equality.
+    equality.
+  Qed.
 
   (* In the second part of this assignment, we will work with a simple language
    * of imperative arithmetic programs that sequentially apply operations
@@ -86,43 +105,69 @@ Module Impl.
    * that running the program [p] should result in, when the
    * initial state is [n].
    *)
-  Fixpoint run (p : Prog) (initState : nat) : nat.
-  Admitted.
+  Fixpoint run (p : Prog) (initState : nat) : nat :=
+    match p with
+    | Done => initState
+    | AddThen n p' => run p' (initState + n)
+    | MulThen n p' => run p' (initState * n)
+    | DivThen n p' => run p' (initState / n)
+    | VidThen n p' => run p' (n / initState)
+    | SetToThen n p' => run p' n
+    end.
 
   Theorem run_Example1 : run Done 0 = 0.
   Proof.
-  Admitted.
+    equality.
+  Qed.
 
   Theorem run_Example2 : run (MulThen 5 (AddThen 2 Done)) 1 = 7.
   Proof.
-  Admitted.
+    equality.
+  Qed.
 
   Theorem run_Example3 : run (SetToThen 3 (MulThen 2 Done)) 10 = 6.
   Proof.
-  Admitted.
+    equality.
+  Qed.
 
   (* Define [numInstructions] to compute the number of instructions
    * in a program, not counting [Done] as an instruction.
    *)
-  Fixpoint numInstructions (p : Prog) : nat.
-  Admitted.
+  Fixpoint numInstructions (p : Prog) : nat :=
+    match p with
+    | Done => 0
+    | AddThen _ p' => 1 + numInstructions p'
+    | MulThen _ p' => 1 + numInstructions p'
+    | DivThen _ p' => 1 + numInstructions p'
+    | VidThen _ p' => 1 + numInstructions p'
+    | SetToThen _ p' => 1 + numInstructions p'
+    end.
 
   Theorem numInstructions_Example :
-    numInstructions (MulThen 5 (AddThen 2 Done)) = 2.
+       numInstructions (MulThen 5 (AddThen 2 Done)) = 2.
   Proof.
-  Admitted.
+    equality.
+  Qed.
 
   (* Define [concatProg] such that [concatProg p1 p2] is the program
    * that first runs [p1] and then runs [p2].
    *)
-  Fixpoint concatProg (p1 p2 : Prog) : Prog.
-  Admitted.
+  Fixpoint concatProg (p1 p2 : Prog) : Prog :=
+    match p1 with
+    | Done => p2
+    | AddThen n p' => AddThen n (concatProg p' p2)
+    | MulThen n p' => MulThen n (concatProg p' p2)
+    | DivThen n p' => DivThen n (concatProg p' p2)
+    | VidThen n p' => VidThen n (concatProg p' p2)
+    | SetToThen n p' => SetToThen n (concatProg p' p2)
+    end.
 
   Theorem concatProg_Example :
        concatProg (AddThen 1 Done) (MulThen 2 Done)
        = AddThen 1 (MulThen 2 Done).
   Proof.
-  Admitted.
+    equality.
+  Qed.
 
   (* Prove that the number of instructions in the concatenation of
    * two programs is the sum of the number of instructions in each
@@ -130,26 +175,33 @@ Module Impl.
    *)
   Theorem concatProg_numInstructions
     : forall (p1 p2 : Prog), numInstructions (concatProg p1 p2)
-                        = numInstructions p1 + numInstructions p2.
+                             = numInstructions p1 + numInstructions p2.
   Proof.
-  Admitted.
+    simplify.
+    induct p1.
+    simplify. equality. simplify.
+    equality. simplify. equality. simplify. equality. simplify. equality. simplify. equality.
+  Qed.
 
   (* Prove that running the concatenation of [p1] with [p2] is
      equivalent to running [p1] and then running [p2] on the
      result. *)
   Theorem concatProg_run
     : forall (p1 p2 : Prog) (initState : nat),
-      run (concatProg p1 p2) initState =
-      run p2 (run p1 initState).
+    run (concatProg p1 p2) initState =
+    run p2 (run p1 initState).
   Proof.
-  Admitted.
+    simplify. induct p1.
+    simplify. equality. simplify. equality. simplify. equality. simplify. equality.
+    simplify. equality. simplify. equality.
+  Qed.
 
   (* Read this definition and understand how division by zero is handled. *)
   Fixpoint runPortable (p : Prog) (state : nat) : bool * nat :=
     match p with
     | Done => (true, state)
-    | AddThen n p => runPortable p (n+state)
-    | MulThen n p => runPortable p (n*state)
+    | AddThen n p => runPortable p (n + state)
+    | MulThen n p => runPortable p (n * state)
     | DivThen n p =>
         if n ==n 0 then (false, state) else
         runPortable p (state/n)
@@ -166,7 +218,11 @@ Module Impl.
   Definition goodProgram1 := AddThen 1 (VidThen 10 Done).
   Example runPortable_good : forall n,
     runPortable goodProgram1 n = (true, 10/(1+n)).
-  Proof. simplify. equality. Qed.
+  Proof. simplify. induct n.
+         simplify. equality. simplify.
+         replace (S (n + 1)) with (S (S n)).
+         equality. linear_arithmetic.
+  Qed.
 
   Definition badProgram1 := AddThen 0 (VidThen 10 Done).
   Example runPortable_bad : let n := 0 in
@@ -176,7 +232,10 @@ Module Impl.
   Definition badProgram2 := AddThen 1 (DivThen 0 Done).
   Example runPortable_bad2 : forall n,
     runPortable badProgram2 n = (false, 1+n).
-  Proof. simplify. equality. Qed.
+  Proof. simplify.
+         replace (n + 1) with (S n).
+         equality. linear_arithmetic.
+  Qed.
 
   (* Prove that running the concatenation [p] using [runPortable]
      coincides with using [run], as long as [runPortable] returns
@@ -184,7 +243,34 @@ Module Impl.
   Lemma runPortable_run : forall p s0 s1,
     runPortable p s0 = (true, s1) -> run p s0 = s1.
   Proof.
-  Admitted.
+    induct p.
+    simplify. equality.
+    simplify.
+    apply IHp.
+    replace (s0 + n) with (n + s0).
+    assumption.
+    linear_arithmetic.
+    simplify.
+    replace (s0 * n) with (n * s0).
+    eapply IHp.
+    assumption.
+    linear_arithmetic.
+    simplify.
+    cases n. simplify.
+    equality. simplify.
+    apply IHp.
+    assumption.
+    simplify.
+    cases s0.
+    simplify.
+    equality.
+    simplify.
+    apply IHp.
+    assumption.
+    simplify.
+    apply IHp.
+    assumption.
+  Qed.
 
   (* The final goal of this pset is to implement [validate : Prog -> bool]
      such that if this function returns [true], the program would not trigger
@@ -220,27 +306,92 @@ Module Impl.
 
   (* HINT 1 (see Pset1Signature.v) *)
 
-  Definition validate (p : Prog) : bool.
-  Admitted.
+  (* The idea here is to use a boolean nz as an overapproximation
+of the runtime state. The nz says "this is 0" or "this is positive".*)
+  Fixpoint validate' (p : Prog) (nz : bool) : bool :=
+    match (p, nz) with
+    | (Done, _) => true
+    | (AddThen 0 p', f) => validate' p' f
+    | (AddThen n p', f) => validate' p' true
+    | (MulThen 0 p', f) => validate' p' false
+    | (MulThen n p', f) => validate' p' f
+    | (DivThen 0 p', f) => false
+    | (DivThen 1 p', f) => validate' p' f
+    | (DivThen n p', f) => validate' p' false
+    | (VidThen n p', false) => false
+    | (VidThen n p', true) => validate' p' false
+    | (SetToThen 0 p', f) => validate' p' false
+    | (SetToThen n p', f) => validate' p' true
+    end.
+
+  Definition validate (p : Prog) : bool := validate' p false.
 
   (* Start by making sure that your solution passes the following tests, and add
    * at least one of your own tests: *)
 
-  Example validate1 : validate goodProgram1 = true. Admitted.
-  Example validate2 : validate goodProgram2 = true. Admitted.
-  Example validate3 : validate goodProgram3 = true. Admitted.
-  Example validate4 : validate goodProgram4 = true. Admitted.
-  Example validate5 : validate goodProgram5 = true. Admitted.
-  Example validate6 : validate goodProgram6 = true. Admitted.
-  Example validate7 : validate goodProgram7 = true. Admitted.
-  Example validateb1 : validate badProgram1 = false. Admitted.
-  Example validateb2 : validate badProgram2 = false. Admitted.
+  Example validate1 : validate goodProgram1 = true.
+  Proof.
+    simplify.
+    equality.
+  Qed.
+
+  Example validate2 : validate goodProgram2 = true.
+  Proof.
+    simplify.
+    equality.
+  Qed.
+
+  Example validate3 : validate goodProgram3 = true.
+  Proof.
+    simplify.
+    equality.
+  Qed.
+
+  Example validate4 : validate goodProgram4 = true.
+  Proof.
+    simplify.
+    equality.
+  Qed.
+
+  Example validate5 : validate goodProgram5 = true.
+  Proof.
+    simplify.
+    equality.
+  Qed.
+
+  Example validate6 : validate goodProgram6 = true.
+  Proof.
+    simplify.
+    equality.
+  Qed.
+
+  Example validate7 : validate goodProgram7 = true.
+  Proof.
+    simplify.
+    equality.
+  Qed.
+
+  Example validateb1 : validate badProgram1 = false.
+  Proof.
+    simplify.
+    equality.
+  Qed.
+
+  Example validateb2 : validate badProgram2 = false.
+  Proof.
+    simplify.
+    equality.
+  Qed.
 
   (* Then, add your own example of a bad program here, and check that `validate`
    * returns `false` on it: *)
 
-  Definition badProgram3 : Prog. Admitted.
-  Example validateb3 : validate badProgram3 = false. Admitted.
+  Definition badProgram3 := AddThen 1 (MulThen 0 (VidThen 10 Done)).
+  Example validateb3 : validate badProgram3 = false.
+  Proof.
+    simplify.
+    equality.
+  Qed.
 
   (* HINTs 2-6 (see Pset1Signature.v)  *)
 
@@ -251,16 +402,216 @@ Module Impl.
    * you need?  Write a short (~10-20 lines) informal proof sketch before
    * proceeding. *)
 
-  (** Proof sketch: **)
-  (* [[Fill in your proof sketch here.]] *)
+  (** Proof sketch:
+
+    The key thing here is to use the auxiliary function validate' (which uses a boolean flag
+    to represent if the state is 0 or positive). Conservative usage of validate' requires that validate
+    is defined by (validate p := validate' p false) because (a priori) we don't know what the initial state
+    will be.
+
+    However, we can pose (validate'_sound) first as a lemma, and utilize assumptions about the state
+    as part of pre-conditions in the lemma:
+
+    (
+      Lemma validate'_sound : forall p s, (validate' p false = true -> runPortable p s = (true, run p s)) /\
+                                  (validate' p true = true /\ s <> 0 -> runPortable p s = (true, run p s)).
+    )
+
+    Here, the basic interpretation is that (forall p s), if (validate' p false = true) then we know (even conservatively!)
+    that (runPortable p s = (true, run p s)). Now, in the second case, if we know (validate' p true = true) --
+    e.g. the case where the flag indicates that the state at this stage of execution is non-zero,
+    we cannot prove anything for all (s), we have to have the additional fact that s <> 0
+    (an easier way to see: if we have (validate' p true = true) and (initState = 0), we can't say anything about (runPortable p s))
+
+    The way that validate'_sound should go is by induction on p.
+    (There's a useful lemma below (validate'_false_implies_true) which I use throughout -- this basically states
+    that, if (validate p = true), it's true for all initial states)
+
+    Throughout the structural induction proof, the inductive hypothesis tends to look the same:
+
+    (
+      IHp : forall s : nat,
+          (validate' p false = true -> runPortable p s = (true, run p s))
+      /\ (validate' p true = true /\ s <> 0 -> runPortable p s = (true, run p s))
+    )
+
+    This is because the inductive data type of programs "wraps" the instantiated (p : Prog, from context). So proving the inductive goal
+    (e.g. AddThen n p) provides an inductive hypothesis like the above.
+
+    All structural cases in the induction will likely also support usage of the (cases n) tactic. This is again due to how we defined our programs.
+    (cases n) will split into (0) and (S _). In certain inductive cases, (0) will lead to contradictions -- which is great, because it allows
+    us to immediately prove sub-goals. In (DivThen n p), (cases n) also supports the (1) case (which is a "no-op" under validate').
+
+    The only time the (cases s) tactic (where s is the state) is required is in (VidThen n p). Again, (0) will lead to a contradiction, (1) is a "no-op".
+
+    One general way to characterize proving each inductive case:
+    the strategy of (simplify, cases n || cases s, rewrite with IHp, equality, linear_arithmetic) mostly works.
+
+    When (validate'_sound) goes through, (validate'_sound) can be used to
+    trivially prove (validate_sound) (by unfolding (validate)).
+
+   **)
+
+  Lemma validate'_false_implies_true : forall p, validate' p false = true -> validate' p true = true.
+  Proof.
+    induct p.
+    simplify.
+    equality.
+    simplify.
+    cases n.
+    eapply IHp.
+    assumption.
+    assumption.
+    simplify.
+    cases n.
+    assumption.
+    apply IHp in H.
+    assumption.
+    simplify.
+    cases n.
+    equality.
+    cases n.
+    eapply IHp.
+    assumption.
+    assumption.
+    simplify.
+    equality.
+    simplify.
+    cases n.
+    assumption.
+    assumption.
+  Qed.
+
+  Lemma validate'_sound : forall p s, (validate' p false = true -> runPortable p s = (true, run p s)) /\
+                                 (validate' p true = true /\ s <> 0 -> runPortable p s = (true, run p s)).
+  Proof.
+    induct p.
+    - simplify. equality.
+    - intros.
+      split.
+      simplify.
+      cases n.
+      eapply IHp in H.
+      replace (0 + s) with (s + 0).
+      apply H.
+      replace (s + 0) with (0 + s).
+      equality.
+      linear_arithmetic.
+      replace (S n + s) with (s + S n).
+      eapply IHp.
+      split.
+      assumption.
+      linear_arithmetic.
+      linear_arithmetic.
+      simplify.
+      cases n.
+      eapply IHp in H.
+      replace (s + 0) with (s).
+      assumption.
+      linear_arithmetic.
+      replace (s + S n) with (S n + s).
+      eapply IHp.
+      split.
+      apply H.
+      linear_arithmetic.
+      linear_arithmetic.
+    - simplify.
+      split.
+      cases n.
+      replace (s * 0) with (0 * s).
+      eapply IHp.
+      linear_arithmetic.
+      replace (s * S n) with (S n * s).
+      eapply IHp.
+      linear_arithmetic.
+      cases n.
+      intros.
+      replace (0 * s) with (s * 0).
+      destruct H.
+      eapply IHp in H.
+      apply H.
+      linear_arithmetic.
+      intros.
+      destruct H.
+      replace (s * S n) with (S n * s).
+      eapply IHp.
+      split.
+      assumption.
+      linear_arithmetic.
+      linear_arithmetic.
+    - split.
+      simplify.
+      cases n.
+      simplify.
+      equality.
+      simplify.
+      cases n.
+      eapply IHp in H.
+      apply H.
+      eapply IHp in H.
+      apply H.
+      simplify.
+      cases n.
+      simplify.
+      equality.
+      simplify.
+      cases n.
+      eapply IHp.
+      split.
+      destruct H.
+      assumption.
+      destruct H.
+      replace (s / 1) with (s).
+      assumption.
+      rewrite Nat.div_1_r.
+      equality.
+      destruct H.
+      eapply IHp in H.
+      apply H.
+    - simplify.
+      split.
+      equality.
+      cases s.
+      simplify.
+      destruct H.
+      equality.
+      simplify.
+      destruct H.
+      eapply IHp in H.
+      apply H.
+    - split.
+      simplify.
+      cases n.
+      eapply IHp in H.
+      apply H.
+      remember (S n).
+      eapply IHp.
+      split.
+      assumption.
+      linear_arithmetic.
+      simplify.
+      cases n.
+      destruct H.
+      eapply IHp in H.
+      apply H.
+      eapply IHp.
+      split.
+      destruct H.
+      assumption.
+      linear_arithmetic.
+  Qed.
 
   (* Now you're ready to write the proof in Coq: *)
-
   Lemma validate_sound : forall p, validate p = true ->
-    forall s, runPortable p s = (true, run p s).
-  Admitted.
+forall s, runPortable p s = (true, run p s).
+  Proof.
+    intros.
+    unfold validate in H.
+    eapply validate'_sound in H.
+    apply H.
+  Qed.
 
-  (* Here is the complete list of commands used in one possible solution:
+(* Here is the complete list of commands used in one possible solution:
     - Search, for example Search (_ + 0).
     - induct, for example induct x
     - simplify
